examples/crypto/cryptobox/Box.PKAE.fst
@@ -20,20 +20,23 @@ module HS = FStar.HyperStack
 
 type rid = FStar.Monotonic.Seq.rid
 
-
-(**
-   Idealisation behaviour of PKAE: 
-     - Requires idealization of both DH and AE
-     - We maintain a global log, that maps a nonce and an AE.key to a message.
-     - When encrypting, we add a new log entry under that nonce AE.key involved.
-*)
-assume val pkae_table_region: (r:MR.rid{ extends r root 
+assume val pkae_afternm_table_region: (r:MR.rid{ extends r root 
 					 /\ is_eternal_region r 
 					 /\ is_below r root 
 					 /\ disjoint r ae_key_region 
-					 /\ disjoint r ae_key_log_region
+					 /\ disjoint r dh_key_log_region
 					 /\ disjoint r id_honesty_table_region
 					 /\ disjoint r id_freshness_table_region
+					 })
+
+assume val pkae_beforenm_table_region: (r:MR.rid{ extends r root 
+					 /\ is_eternal_region r 
+					 /\ is_below r root 
+					 /\ disjoint r ae_key_region 
+					 /\ disjoint r dh_key_log_region
+					 /\ disjoint r id_honesty_table_region
+					 /\ disjoint r id_freshness_table_region
+					 /\ disjoint r pkae_afternm_table_region
 					 })
 					 
 //let pkae_table_region = new_region root
@@ -43,14 +46,14 @@ type pkae_afternm_table_key = (nonce*(i:id{AE_id? i}))
 type pkae_afternm_table_value = (protected_pkae_plain)
 type pkae_afternm_table_range = fun pkae_afternm_table_key -> pkae_afternm_table_value
 type pkae_afternm_table_inv (f:MM.map' pkae_afternm_table_key pkae_afternm_table_range) = True
-assume val pkae_afternm_table: MM.t pkae_table_region pkae_afternm_table_key pkae_afternm_table_range pkae_afternm_table_inv
+assume val pkae_afternm_table: MM.t pkae_afternm_table_region pkae_afternm_table_key pkae_afternm_table_range pkae_afternm_table_inv
 //let pkae_afternm_table = MM.alloc #pkae_table_region #pkae_table_key #pkae_table_range #pkae_table_inv
 
 type pkae_beforenm_table_key = i:id{AE_id? i}
 type pkae_beforenm_table_value = (AE.key)
 type pkae_beforenm_table_range = fun (i:pkae_beforenm_table_key) -> (k:pkae_beforenm_table_value{AE.get_index k = i})
 type pkae_beforenm_table_inv (f:MM.map' pkae_beforenm_table_key pkae_beforenm_table_range) = True
-assume val pkae_beforenm_table:  MM.t pkae_table_region pkae_beforenm_table_key pkae_beforenm_table_range pkae_beforenm_table_inv
+assume val pkae_beforenm_table:  MM.t pkae_beforenm_table_region pkae_beforenm_table_key pkae_beforenm_table_range pkae_beforenm_table_inv
 //let pkae_beforenm_table = MM.alloc #pkae_table_region #pkae_table_key #pkae_table_range #pkae_table_inv
 
 
@@ -60,13 +63,15 @@ noeq abstract type pkae_pkey (pk_id:id{DH_id? pk_id}) =
 noeq abstract type pkae_skey (sk_id:id{DH_id? sk_id}) =
   | SKey: dh_sk:dh_skey{DH.sk_get_index dh_sk=sk_id} -> pkae_pk:pkae_pkey sk_id -> pkae_skey sk_id
 
-// Require a fresh id here?
 val keygen: #(i:id{DH_id? i}) -> ST (pkae_pkey i * pkae_skey i)
   (requires (fun h0 -> 
   fresh i h0
   /\ fixed i
   ))
-  (ensures (fun h0 res h1 -> True ))
+  (ensures (fun h0 res h1 -> 
+    unfresh i
+    /\ modifies (Set.singleton id_freshness_table_region) h0 h1
+  ))
 let keygen #i =
   let (dh_pk, dh_sk) = DH.keygen #i in
   let pkae_pk = PKey #i dh_pk in
@@ -75,6 +80,10 @@ let keygen #i =
 
 type c = AE.cipher
 
+let log_invariant (h:mem) = 
+  forall (k:AE.key) (n:nonce). let k_log = get_logGT k in (MM.fresh k_log n h <==> MM.fresh pkae_afternm_table (n,AE.get_index k) h)
+
+#set-options "--z3rlimit 15"
 val encrypt_beforenm: #(pk_id:id{DH_id? pk_id /\ fixed pk_id}) -> 
 	              #(sk_id:id{DH_id? sk_id /\ fixed sk_id}) -> 
 	              pk:pkae_pkey pk_id -> 
@@ -83,18 +92,40 @@ val encrypt_beforenm: #(pk_id:id{DH_id? pk_id /\ fixed pk_id}) ->
   (requires (fun h0 -> 
     let i = generate_ae_id pk_id sk_id in
     fixed i
+    /\ honest i ==> (~(MR.witnessed(MM.defined dh_key_log i) ==> ~(fresh i h0)))
+    /\ log_invariant h0
   ))
   (ensures (fun h0 k h1 -> 
     let i = generate_ae_id pk_id sk_id in
-    let k_log = leak_logGT k in
-    AE.get_index k = i
+    let regions_modified_dishonest:Set.set (r:HH.rid) = (Set.singleton id_freshness_table_region) in
+    let regions_modified_honest = Set.union regions_modified_dishonest (Set.singleton dh_key_log_region) in
+    let k_log = get_logGT k in
+    (PlainDH.ae_key_get_index k = i)
+    /\ (
+        ( (honest i)
+    	    ==> (modifies regions_modified_honest h0 h1
+    	       /\ MR.witnessed (MM.contains dh_key_log i k) 
+    	      )
+        )
+        \/ 
+    	( (dishonest i \/ ~Flags.prf_odh)
+    	    ==> (modifies regions_modified_dishonest h0 h1
+    	       /\ leak_key k = DH.prf_odhT sk.dh_sk pk.dh_pk
+    	      )
+        )
+      )
     /\ MR.m_contains k_log h1
+    /\ modifies regions_modified_honest h0 h1
+    /\ (forall k. let k_region = get_regionGT k in
+      equal_on (Set.singleton k_region) h0.h h1.h)
+    /\ (let k_region = get_regionGT k in
+      equal_on (Set.singleton pkae_afternm_table_region) h0.h h1.h)
+    /\ log_invariant h1
   ))
 let encrypt_beforenm #pk_id #sk_id pk sk =
-  MR.m_recall pkae_beforenm_table;
-  let i = generate_ae_id pk_id sk_id in
-  let ae_honest_i = honestST i in
+  MR.m_recall pkae_afternm_table;
   let k = prf_odh sk.dh_sk pk.dh_pk in
+  recall_log k;
   k
 
 
@@ -105,17 +136,16 @@ val encrypt_afternm: k:AE.key ->
 		     p:protected_pkae_plain{PlainPKAE.get_index p = AE.get_index k} ->
 		     ST c
   (requires (fun h0 -> 
-    let k_log = leak_logGT k in
+    let k_log = get_logGT k in
     MM.fresh pkae_afternm_table (n,AE.get_index k) h0
-    /\ MM.fresh (leak_logGT k) n h0
     /\ MR.m_contains k_log h0
     /\ MR.m_contains pkae_afternm_table h0
+    /\ log_invariant h0
   ))
   (ensures (fun h0 c h1 -> 
     let i = AE.get_index k in
-    let k_log = leak_logGT k in
-    let k_raw = leak_keyGT k in
-    MR.m_contains k_log h1
+    let k_log = get_logGT k in
+    let k_raw = get_keyGT k in
     ///\ (
     //	( (dishonest i \/ ~(b2t pkae))
     //	    ==> c = CoreCrypto.aead_encryptT AES_128_CCM k_raw n empty_bytes (PlainPKAE.repr p))
@@ -123,17 +153,24 @@ val encrypt_afternm: k:AE.key ->
     //    ( (honest i /\ b2t ae_ind_cca)
     //	    ==> c = CoreCrypto.aead_encryptT AES_128_CCM k_raw n empty_bytes (createBytes (PlainPKAE.length p) 0z) )
     //  )
-    /\ (dishonest i \/ honest i)
+    (dishonest i \/ honest i)
     /\ MR.witnessed (MM.contains k_log n (c,ae_message_wrap p))
     /\ MR.witnessed (MM.contains pkae_afternm_table (n,i) p)
+    /\ log_invariant h0
   ))
 let encrypt_afternm k n p =
+//  let h0 = ST.get() in
+//  assert(
+//    let k_log = get_logGT k in
+//    MM.fresh k_log n h0);
+//  admit();
   let ae_i = AE.get_index k in
   let ae_m = ae_message_wrap #ae_i p in
   MM.extend pkae_afternm_table (n,ae_i) p;
   AE.encrypt #ae_i n k ae_m
+  
 
-
+#set-options "--z3rlimit 15"
 val encrypt: #(pk_id:id{DH_id? pk_id}) -> 
 	     #(sk_id:id{DH_id? sk_id}) -> 
 	     pk:pkae_pkey pk_id{fixed pk_id} -> 
@@ -143,17 +180,22 @@ val encrypt: #(pk_id:id{DH_id? pk_id}) ->
 	     -> ST c 
   (requires (fun h0 ->
     let i = generate_ae_id pk_id sk_id in
-    let k_log = leak_logGT k in
     fixed i
-    /\ MR.m_contains k_log h0
-    /\ MR.m_contains pkae_afternm_table
-    /\ MR.m_contains pkae_beforenm_table
+    /\ MR.m_contains pkae_afternm_table h0
+    /\ (honest i ==> (~(MR.witnessed(MM.defined dh_key_log i) ==> ~(fresh i h0))))
+    /\ MM.fresh pkae_afternm_table (n,i) h0
+    // Make sure that log_invariant holds
+    /\ MM.fresh pkae_afternm_table (n,i) h0
+    /\ log_invariant h0
   ))
-  (ensures (fun h0 c h1 -> True ))
+  (ensures (fun h0 c h1 -> 
+    log_invariant h1
+  ))
 let encrypt #pk_id #sk_id pkae_pk pkae_sk n p =
   let k = encrypt_beforenm #pk_id #sk_id pkae_pk pkae_sk in
   let c = encrypt_afternm k n p in
   c
+
 
 // Implement decrypt_beforenm and decrypt_afternm
 // - add similar specification as in AE and in PKAE.encrypt..
